LambdaLab/ParserExperimental1/Biparser/Mixfix/Render.lean
@@ -24,12 +24,15 @@ def Tree.render {G : Grammar} : {p : Nat} → Tree G p → (Nat → Nat) → Nat
          ++ (Tree.render t f (i + 1)).1
          ++ gapRp.render ((), rpVal) (f (Tree.render t f (i + 1)).2, ()),
        (Tree.render t f (i + 1)).2 + 1)
-  | _, .op k hk _ l r,  f, i =>
+  | _, .op k hk _ _ l r,  f, i =>
       ((Tree.render l f i).1
          ++ (gapOpGap G k hk).render ((), opVal G k hk, ())
               (f (Tree.render l f i).2, (), f ((Tree.render l f i).2 + 1))
          ++ (Tree.render r f ((Tree.render l f i).2 + 2)).1,
        (Tree.render r f ((Tree.render l f i).2 + 2)).2)
+  | _, .pre k hk _ _ e,   f, i =>
+      ((opGap G k hk).render (opVal G k hk, ()) ((), f i) ++ (Tree.render e f (i + 1)).1,
+       (Tree.render e f (i + 1)).2)
 
 #eval String.ofList (Tree.render sampleTree (fun _ => 0) 0).1        -- "a + b * c"
 #eval String.ofList (Tree.render sampleTree (fun i => i) 0).1        -- widening gaps
